puliendo ejemplos

ejemplos/mcd/mcd.dfy
@@ -17,18 +17,16 @@ method test_es_el_mcd_numeros_chicos(){
     assert es_el_mcd(1, 49163, 9113);
 }
 
-predicate invariante(d: int, m': int, n': int, r: int) {
+predicate invariante(d: int, m': int, n': int) {
     && es_el_mcd(d, m', n')
-    && r == m' % n'
-    && (r == 0 ==> d == n')
+    && (m' % n' == 0 ==> d == n')
 }
 
-method {:axiom} inicializacion(ghost d: int, m: int, n: int) returns (m': int, n': int, r: int)
+method {:axiom} inicializacion(ghost d: int, m: int, n: int) returns (m': int, n': int)
     requires 0 < n <= m
     requires es_el_mcd(d, m, n)
-    ensures invariante(d, m', n', r)
+    ensures invariante(d, m', n')
 {
-    r := m % n;
     m' := m;
     n' := n;
 }
@@ -38,18 +36,17 @@ lemma {:axiom} mcd_del_modulo(d:int, m:int, n:int)
     requires n > 0
     ensures es_el_mcd(d, n, m % n)
 
-method {:axiom} cuerpo(ghost d: int, m: int, n: int, r: int) returns (m': int, n': int, r': int)
-    requires r > 0
-    requires invariante(d, m, n, r)
-    ensures invariante(d, m', n', r')
-    ensures r' < r
+method {:axiom} cuerpo(ghost d: int, m: int, n: int) returns (m': int, n': int)
+    requires invariante(d, m, n)
+    ensures invariante(d, m', n')
+    ensures m' % n' < m % n
 {
     assert es_el_mcd(d, n, m % n) by {
         mcd_del_modulo(d, m, n);
     }
+    var r := m % n;
     m' := n;
     n' := r;
-    r' := m' % n';
 }
 
 lemma {:axiom} existe_un_mcd(m:int, n:int)
@@ -63,13 +60,13 @@ method maximo_comun_divisor(m: int, n: int) returns (mcd: int)
         existe_un_mcd(m, n);
     }
     ghost var d: int :| es_el_mcd(d, m, n);
-    var m': int, n': int, r: int;
-    m', n', r := inicializacion(d, m, n);
-    while (r > 0)
-        decreases r
-        invariant invariante(d, m', n', r)
+    var m': int, n': int;
+    m', n' := inicializacion(d, m, n);
+    while (m' % n' > 0)
+        decreases m' % n'
+        invariant invariante(d, m', n')
     {
-         m', n', r := cuerpo(d, m', n', r);
+         m', n' := cuerpo(d, m', n');
     }
     return n';
 }
